thesis/algebra/Temporal_Faults_Algebra.thy
@@ -75,7 +75,6 @@ class temporal_faults_algebra_mixed_ops = temporal_faults_algebra_trans +
   assumes inf_xbefore_equiv_sups_xbefore: "tempo2 a \<Longrightarrow> inf a (xbefore b c) = 
     sup (xbefore (inf a b) c) (xbefore b (inf a c))"
 
-
 class temporal_faults_algebra = temporal_faults_algebra_mixed_ops
 
 subsection {* Theorems in the context of \ac{algebra} *}
